unverified/interp.hs
@@ -78,7 +78,7 @@ put s = M_st_ex (\s' -> (s, Rval ()))
 raise :: Error_result -> M_st_ex a b
 raise err = M_st_ex (\s -> (s, Rerr err))
 
-handle :: M_st_ex s a -> (Integer -> M_st_ex s a) -> M_st_ex s a
+handle :: M_st_ex s a -> (V -> M_st_ex s a) -> M_st_ex s a
 handle v f =
   M_st_ex (\s -> case run_M_st_ex v s of
                    (s, Rerr (Rraise v)) -> run_M_st_ex (f v) s
@@ -230,7 +230,7 @@ do_app s env' op v1 v2 =
             Nothing -> Nothing
       (Opn op pos, Litv (IntLit n1), Litv (IntLit n2)) ->
         if (op == Divide || op == Modulo) && n2 == 0 then
-          Just (s, env', Raise (Con (Just (Short (ConN "Div")) [])))
+          Just (s, env', Raise (Con (Just (Short (ConN "Div" dummy_pos))) [] dummy_pos))
         else
           Just (s, env',Lit (IntLit (opn_lookup op n1 n2)) pos)
       (Opb op pos, Litv (IntLit n1), Litv (IntLit n2)) ->
@@ -238,7 +238,7 @@ do_app s env' op v1 v2 =
       (Equality pos, v1, v2) ->
         case do_eq v1 v2 of
             Eq_type_error -> Nothing
-            Eq_closure -> Just (s, env', Raise (Con (Just (Short (ConN "Eq")) [])))
+            Eq_closure -> Just (s, env', Raise (Con (Just (Short (ConN "Eq" dummy_pos))) [] dummy_pos))
             Eq_val b -> Just (s, env', Lit (Bool b) pos)
       (Opassign pos, (Loc lnum), v) ->
         case store_assign lnum v s of
@@ -308,7 +308,7 @@ run_eval menv cenv env (If e1 e2 e3) =
            Just e' -> run_eval menv cenv env e'
 run_eval menv cenv env (Mat e pes) =
    do v <- run_eval menv cenv env e;
-      run_eval_match menv cenv env v pes (Conv (Just (Short "Bind") []))
+      run_eval_match menv cenv env v pes (Conv (Just (Short (ConN "Bind" dummy_pos))) [])
 run_eval menv cenv env (Let x e1 e2) =
    do v1 <- run_eval menv cenv env e1;
       run_eval menv cenv (bind x v1 env) e2
@@ -353,7 +353,7 @@ run_eval_dec mn menv cenv st env (Dlet p e pos) =
          (st', Rval v) ->
            (case pmatch cenv st' p v emp of
                 Match env' -> (st', Rval (emp, env'))
-                No_match -> (st', Rerr (Rraise (Conv (Just (Short "Bind") []))))
+                No_match -> (st', Rerr (Rraise (Conv (Just (Short (ConN "Bind" dummy_pos))) [])))
                 Match_type_error -> (st', Rerr Rtype_error))
          (st', Rerr e) -> (st', Rerr e)
   else
