semantics/BigStepScript.sml
@@ -435,7 +435,21 @@ evaluate_dec mn menv cenv s env (Dtype tds) (s, Rval (build_tdefs mn tds, emp)))
 
 (! mn menv cenv env tds s. ( ~  (check_dup_ctors mn cenv tds))
 ==>
-evaluate_dec mn menv cenv s env (Dtype tds) (s, Rerr Rtype_error))`;
+evaluate_dec mn menv cenv s env (Dtype tds) (s, Rerr Rtype_error))
+
+/\
+
+(! mn menv cenv env cn ts s.
+(lookup (mk_id mn cn) cenv = NONE)
+==>
+evaluate_dec mn menv cenv s env (Dexn cn ts) (s, Rval (bind (mk_id mn cn) ( LENGTH ts, TypeExn) emp, emp)))
+
+/\
+
+(! mn menv cenv env cn ts s.
+(lookup (mk_id mn cn) cenv <> NONE)
+==>
+evaluate_dec mn menv cenv s env (Dexn cn ts) (s, Rerr Rtype_error))`;
 
 val _ = Hol_reln `
 
@@ -531,6 +545,7 @@ val _ = Define `
       Dlet p e => ALL_DISTINCT (pat_bindings p []) /\ e_diverges menv cenv st env e
     | Dletrec funs => F
     | Dtype tds => F
+    | Dexn cn ts => F
   )))`;
 
 
